examples/mod3.c
@@ -1,10 +1,10 @@
 unsigned long long delta(unsigned long long, unsigned long long);
-_Bool accept(unsigned long long);
+unsigned long long accept(unsigned long long);
 unsigned long long run(unsigned long long *, unsigned long long);
 int $12(void);
 unsigned long long const table[6] = { 0LL, 2LL, 1LL, 0LL, 2LL, 1LL, };
 
-unsigned int const atable[3] = { 0, 0, 1, };
+unsigned long long const atable[3] = { 1LL, 1LL, 0LL, };
 
 unsigned long long delta(unsigned long long $6, unsigned long long $7)
 {
@@ -15,7 +15,7 @@ unsigned long long delta(unsigned long long $6, unsigned long long $7)
   }
 }
 
-_Bool accept(unsigned long long $6)
+unsigned long long accept(unsigned long long $6)
 {
   if ($6 < 3LLU) {
     return *(atable + $6);
