examples/traffic.c
@@ -1,5 +1,5 @@
 unsigned long long delta(unsigned long long, unsigned long long);
-unsigned long long accept(unsigned long long);
+unsigned long long output(unsigned long long);
 unsigned long long run(unsigned long long *, unsigned long long);
 int $12(void);
 unsigned long long const table[8] = { 3LL, 3LL, 0LL, 3LL, 1LL, 3LL, 2LL, 3LL,
@@ -16,7 +16,7 @@ unsigned long long delta(unsigned long long $6, unsigned long long $7)
   }
 }
 
-unsigned long long accept(unsigned long long $6)
+unsigned long long output(unsigned long long $6)
 {
   if ($6 < 4LLU) {
     return *(atable + $6);
