theories/compiler/dfa.v
@@ -1,7 +1,7 @@
 From lstar Require Import Automata.
 From compcert Require Import AST Clight Ctypes Integers Cop Maps.
-From Transmogrifier Require Import Monads.
-From Stdlib Require Import String List ZArith.
+From Transmogrifier Require Import Monads moore.
+From Stdlib Require Import String List ZArith Bool.
 Import ListNotations.
 Open Scope result_scope.
 Open Scope string_scope.
@@ -37,278 +37,32 @@ Module DFACompiler (s : Symbol) (DFA : DFAType s).
 
 Import DFA.
 
-(* Identifier allocation *)
+Module Out <: Output.
+  Definition t := bool.
+  Definition eq_dec := bool_dec.
+  Definition enum := [true; false].
+  Theorem t_enumerable : forall x : bool, In x enum.
+  Proof. unfold enum. intros [|]. now left. right. now left. Qed.
+End Out.
 
-Record idents : Type := {
-  id_delta  : ident;
-  id_accept : ident;
-  id_q0     : ident;
-  id_table  : ident;
-  id_atable : ident;
-  id_q      : ident;
-  id_s      : ident;
-  id_w      : ident;
-  id_len    : ident;
-  id_i      : ident;
-  id_run    : ident;
-  id_main   : ident
-}.
+Module Moore <: MooreType s Out.
+  Record t (state : Type) : Type := {
+        transition : state -> s.t -> state;
+        initial : state;
+        output : state -> bool;
+        states : list state;
+        states_complete : forall w, In (fold_left transition w initial) (states)
+    }.
 
-Definition alloc_idents (base : ident) : idents := {|
-  id_delta  := base;
-  id_accept := 1 + base;
-  id_q0     := 2 + base;
-  id_table  := 3 + base;
-  id_atable := 4 + base;
-  id_q      := 5 + base;
-  id_s      := 6 + base;
-  id_w      := 7 + base;
-  id_len    := 8 + base;
-  id_i      := 9 + base;
-  id_run    := 10 + base;
-  id_main   := 11 + base
-|}%positive.
+  Definition run {state : Type} (dfa : t state) (s : list s.t) : state :=
+        fold_left dfa.(transition state) s dfa.(initial state).
 
-(* Types *)
+  Theorem run_in_states : forall {state : Type} (d : t state) (w : list s.t),
+        In (run d w) (states state d).
+  Proof. intros. apply states_complete. Qed.
+End Moore.
 
-Definition tlong : type := Tlong Unsigned noattr.
-Definition tuint : type := Tint I32 Unsigned noattr.
-Definition tint : type := Tint I32 Signed noattr.
-Definition tbool : type := Tint IBool Unsigned noattr.
+Module MooreCompiler := MooreCompiler s Out Moore.
+Include MooreCompiler.
 
-Section compiler.
-Variable state : Type.
-Variable dfa : DFA.t state.
-Variable state_eq_dec : forall x y : state, {x = y} + {x <> y}.
-
-(* Return value for out-of-bounds transition inputs *)
-Definition sink_index : Z := Z.of_nat (length dfa.(states _)).
-
-Fixpoint index_of {X : Type} (eq_dec : forall x y : X, {x = y} + {x <> y})
-                  (target : X) (l : list X) (idx : Z) : option Z :=
-  match l with
-  | [] => None
-  | h :: t => if eq_dec target h then Some idx else index_of eq_dec target t (Z.succ idx)
-  end.
-
-Definition enumerate {X : Type} (l : list X) : list (Z * X) :=
-  combine (map Z.of_nat (seq 0 (length l))) l.
-
-Definition state_table : list (Z * state) := enumerate dfa.(states _).
-Definition sym_table   : list (Z * s.t)   := enumerate s.enum.
-
-Definition compiled_enum {X : Type} (l : list X) : list Clight.expr :=
-  map (fun '(i, _) => Econst_long (Int64.repr i) tlong) (enumerate l).
-
-Definition compiled_sigma : list Clight.expr := compiled_enum s.enum.
-Definition compiled_Q     : list Clight.expr := compiled_enum dfa.(states _).
-
-Definition q0_index : Z :=
-  match index_of state_eq_dec dfa.(initial _) dfa.(states _) 0 with
-  | Some i => i
-  | None => sink_index
-  end.
-
-Definition compiled_q0 : Clight.expr :=
-  Econst_long (Int64.repr q0_index) tlong.
-
-(*  delta
-
-    Emitted as a 2D lookup table *)
-
-Definition nsyms : Z := Z.of_nat (length s.enum).
-Definition nstates : Z := Z.of_nat (length dfa.(states _)).
-
-(* The transition table, flattened row-major: entry [q * |Sigma| + s]
-   holds the index of [delta q s]. Rows are indexed by state, columns
-   by symbol. *)
-Definition table_entry (q : state) (sym : s.t) : Z :=
-  match index_of state_eq_dec (dfa.(transition _) q sym) dfa.(states _) 0 with
-  | Some i => i
-  | None => sink_index
-  end.
-
-Definition table_row (q : state) : list init_data :=
-  map (fun '(_, sym) => Init_int64 (Int64.repr (table_entry q sym))) sym_table.
-
-Definition table_init : list init_data :=
-  flat_map (fun '(_, q) => table_row q) state_table.
-
-Definition table_type : type :=
-  Tarray tlong (nstates * nsyms) noattr.
-
-Definition compile_table : globvar type := {|
-  gvar_info     := table_type;
-  gvar_init     := table_init;
-  gvar_readonly := true;
-  gvar_volatile := false
-|}.
-
-(* unsigned long long delta(unsigned long long q, unsigned long long s) {
-     if (q < |Q| && s < |Sigma|)
-       return table[q * |Sigma| + s];
-     else
-       return |Q|;
-   } *)
-Definition lt_test (v : ident) (k : Z) : Clight.expr :=
-  Ebinop Olt (Etempvar v tlong) (Econst_long (Int64.repr k) tlong) tint.
-
-Definition table_index (ids : idents) : Clight.expr :=
-  Ebinop Oadd
-    (Ebinop Omul (Etempvar ids.(id_q) tlong) (Econst_long (Int64.repr nsyms) tlong) tlong)
-    (Etempvar ids.(id_s) tlong)
-    tlong.
-
-Definition compile_delta (ids : idents) : Clight.fundef :=
-  let body :=
-    Sifthenelse
-      (Ebinop Oand (lt_test ids.(id_q) nstates) (lt_test ids.(id_s) nsyms) tint)
-      (Sreturn (Some
-        (Ederef
-          (Ebinop Oadd (Evar ids.(id_table) table_type) (table_index ids)
-            (Tpointer tlong noattr))
-          tlong)))
-      (Sreturn (Some (Econst_long (Int64.repr sink_index) tlong)))
-  in
-  Internal {|
-    fn_return   := tlong;
-    fn_callconv := AST.cc_default;
-    fn_params   := [(ids.(id_q), tlong); (ids.(id_s), tlong)];
-    fn_vars     := [];
-    fn_temps    := [];
-    fn_body     := body
-  |}.
-
-Definition delta_type : type :=
-  Tfunction [tlong; tlong] tlong AST.cc_default.
-
-(* accept *)
-
-Definition accept_entry (q : state) : Z :=
-  if dfa.(accept _) q then 1 else 0.
-
-Definition atable_type : type := Tarray tuint nstates noattr.
-
-Definition atable_init : list init_data :=
-  map (fun '(_, q) => Init_int32 (Int.repr (accept_entry q))) state_table.
-
-Definition compile_atable : globvar type := {|
-  gvar_info     := atable_type;
-  gvar_init     := atable_init;
-  gvar_readonly := true;
-  gvar_volatile := false
-|}.
-
-(* _Bool accept(unsigned long long q) {
-     if (q < |Q|) return atable[q]; else return 0;
-   } *)
-Definition compile_accept (ids : idents) : Clight.fundef :=
-  let body :=
-    Sifthenelse (lt_test ids.(id_q) nstates)
-      (Sreturn (Some
-        (Ederef
-          (Ebinop Oadd (Evar ids.(id_atable) atable_type) (Etempvar ids.(id_q) tlong)
-            (Tpointer tuint noattr))
-          tuint)))
-      (Sreturn (Some (Ecast (Econst_int Int.zero tuint) tbool)))
-  in
-  Internal {|
-    fn_return   := tbool;
-    fn_callconv := AST.cc_default;
-    fn_params   := [(ids.(id_q), tlong)];
-    fn_vars     := [];
-    fn_temps    := [];
-    fn_body     := body
-  |}.
-
-(* q0 *)
-
-Definition compile_q0 : globvar type := {|
-  gvar_info     := tlong;
-  gvar_init     := [Init_int64 (Int64.repr q0_index)];
-  gvar_readonly := true;
-  gvar_volatile := false
-|}.
-
-(* run *)
-
-Definition w_type : type :=
-  Tpointer tlong noattr.
-
-(* int run(int *w, int len) {
-     int i = 0;
-     int q = q0;
-     while(i < len) {
-       q = delta(q, w[i]);
-       i++;
-     }
-     return q;
-   } *)
-Definition run_body (ids : idents) : statement :=
-  Ssequence
-    (Sifthenelse
-      (Ebinop Olt (Etempvar ids.(id_i) tlong) (Etempvar ids.(id_len) tlong) tint)
-      Sskip Sbreak)
-    (Ssequence
-      (Scall (Some ids.(id_q)) (Evar ids.(id_delta) delta_type)
-         [ Etempvar ids.(id_q) tlong;
-           Ederef (Ebinop Oadd (Etempvar ids.(id_w) w_type)
-                     (Etempvar ids.(id_i) tlong) w_type) tlong ])
-      (Sset ids.(id_i)
-        (Ebinop Oadd (Etempvar ids.(id_i) tlong) (Econst_long (Int64.repr 1) tlong) tlong))).
-
-Definition run_loop (ids : idents) : statement := Sloop (run_body ids) Sskip.
-
-Definition run_prologue (ids : idents) : statement :=
-  Ssequence
-    (Sset ids.(id_i) (Econst_long (Int64.repr 0) tlong))
-    (Sset ids.(id_q) compiled_q0).
-
-Definition compile_run (ids : idents) : Clight.fundef :=
-  let final_body :=
-    Ssequence
-      (Ssequence (run_prologue ids) (run_loop ids))
-      (Sreturn (Some (Etempvar ids.(id_q) tlong))) in
-  Internal {|
-    fn_return   := tlong;
-    fn_callconv := AST.cc_default;
-    fn_params   := [(ids.(id_w), w_type); (ids.(id_len), tlong)];
-    fn_vars     := [];
-    fn_temps    := [(ids.(id_i), tlong); (ids.(id_q), tlong)];
-    fn_body     := final_body
-  |}.
-
-(* Program assembly *)
-
-Definition tint32s : type := Tint I32 Signed noattr.
-
-Definition compile_main (ids : idents) : Clight.fundef :=
-  Internal {|
-    fn_return   := tint32s;
-    fn_callconv := AST.cc_default;
-    fn_params   := [];
-    fn_vars     := [];
-    fn_temps    := [];
-    fn_body     := Sreturn (Some (Econst_int Int.zero tint32s))
-  |}.
-
-Definition compile_program (base : ident) : result Clight.program :=
-  let ids := alloc_idents base in
-  let defs : list (ident * globdef Clight.fundef type) :=
-    [ (ids.(id_table),  Gvar (compile_table));
-      (ids.(id_atable), Gvar (compile_atable));
-      (ids.(id_delta),  Gfun (compile_delta ids));
-      (ids.(id_accept), Gfun (compile_accept ids));
-      (ids.(id_q0),     Gvar (compile_q0));
-      (ids.(id_run),    Gfun (compile_run ids));
-      (ids.(id_main),   Gfun (compile_main ids)) ] in
-  match Ctypes.make_program [] defs
-          [ids.(id_delta); ids.(id_accept); ids.(id_q0); ids.(id_table);
-           ids.(id_atable); ids.(id_run); ids.(id_main)]
-          ids.(id_main) with
-  | Errors.OK p => return p
-  | Errors.Error msg => fail E_msg "make_program failed"
-  end.
-
-End compiler.
 End DFACompiler.
